Implement most of the transfer function methods for pmaps.

src/PMapAbstractDomain.v
@@ -1,10 +1,12 @@
 From Coq Require Import ssreflect ssrfun ssrbool.
-From PolyAI Require Export Presburger AbstractDomain RelationalAbstractDomain LSSA.
+From PolyAI Require Export Presburger AbstractDomain RelationalAbstractDomain LSSA RelationalTransferFunction.
+From mathcomp.ssreflect Require Export seq.
 
 Section PMapAbstractDomain.
 
   Context {PMap PSet PwAff: eqType}
-          {PI: PresburgerImpl PMap PSet PwAff}.
+          {PI: PresburgerImpl PMap PSet PwAff}
+          (prog: Program).
 
   Definition concrete_state := prod_eqType RegisterMap RegisterMap.
 
@@ -27,18 +29,18 @@ Section PMapAbstractDomain.
   Qed.
 
   Theorem gamma_pmap_top :
-    forall x, In concrete_state (gamma_pmap universe_map) x.
+    forall x, Ensembles.In concrete_state (gamma_pmap universe_map) x.
   Proof.
     move => x.
-    rewrite /gamma_pmap /In.
+    rewrite /gamma_pmap /Ensembles.In.
       by auto_presburger.
   Qed.
 
   Theorem gamma_pmap_bot :
-    forall x, ~ In concrete_state (gamma_pmap empty_map) x.
+    forall x, ~ Ensembles.In concrete_state (gamma_pmap empty_map) x.
   Proof.
     move => x.
-    rewrite /gamma_pmap /In.
+    rewrite /gamma_pmap /Ensembles.In.
       by auto_presburger.
   Qed.
 
@@ -78,19 +80,19 @@ Section PMapAbstractDomain.
     }.
 
   Theorem pmap_id_relation_spec :
-    forall x0 x1, In _ (gamma id_map) (x0, x1) <-> x0 = x1.
+    forall x0 x1, Ensembles.In _ (gamma id_map) (x0, x1) <-> x0 = x1.
   Proof.
     move => x0 x1.
-    rewrite /In /gamma /= /gamma_pmap /= id_map_spec.
+    rewrite /Ensembles.In /gamma /= /gamma_pmap /= id_map_spec.
       by split; autossr.
   Qed.
 
   Theorem pmap_compose_relation_spec :
-    forall a1 a2 x0 x2, In _ (gamma (map_apply_range a1 a2)) (x0, x2) <->
-                   exists x1, In _ (gamma a1) (x0, x1) /\ In _ (gamma a2) (x1, x2).
+    forall a1 a2 x0 x2, Ensembles.In _ (gamma (map_apply_range a1 a2)) (x0, x2) <->
+                   exists x1, Ensembles.In _ (gamma a1) (x0, x1) /\ Ensembles.In _ (gamma a2) (x1, x2).
   Proof.
     move => a1 a2 x0 x2.
-    rewrite /In /gamma /= /gamma_pmap /=.
+    rewrite /Ensembles.In /gamma /= /gamma_pmap /=.
       by apply map_apply_range_spec.
   Qed.
 
@@ -109,5 +111,197 @@ Section PMapAbstractDomain.
       transitive_closure_ge_step := transitive_closure_map_ge_step;
       transitive_closure_eq_compose := transitive_closure_map_eq_compose;
     }.
+
+  Definition pmap_set_out_var_const (m: PMap) (v: string) (c: Z) :=
+  let c_map := Presburger.eq_map (pw_aff_from_aff (AConst 0)) (pw_aff_from_aff (AVar v)) (pw_aff_from_aff (AConst 0)) (pw_aff_from_aff (AConst c)) in
+  let m := map_project_out_out m v in
+  intersect_map c_map m.
+
+  Theorem pmap_set_out_var_const_spec (m: PMap) :
+    forall x0 x1, Ensembles.In _ (gamma m) (x0, x1) ->
+             forall v c, Ensembles.In _ (gamma (pmap_set_out_var_const m v c)) (x0, (v !-> c ; x1)).
+  Proof.
+    move => x0 x1 Heval v c.
+    rewrite /gamma /= /gamma_pmap /Ensembles.In /= /pmap_set_out_var_const.
+    simpl_presburger.
+    apply map_project_out_out_spec.
+    exists (x1 v). by simpl_map.
+  Qed.
+
+  Theorem pmap_set_out_var_const_tf_sound :
+    forall v c R R', inst_step (Const v c) R R' ->
+                 forall m R_begin, Ensembles.In _ (gamma m) (R_begin, R) ->
+                              Ensembles.In _ (gamma (pmap_set_out_var_const m v c)) (R_begin, R').
+  Proof.
+    move => v c R R' Hstep m R_begin HIn.
+    inversion Hstep. subst.
+      by apply pmap_set_out_var_const_spec.
+  Qed.
+
+  (* Transfer function for binary arithmetic operation *)
+  Definition binop_to_pwaff (res: vid) (opc: BinArithOpCode) (op1 op2: vid) :=
+    match opc with
+    | OpAdd => pw_aff_from_aff (APlus (AVar op1) (AVar op2))
+    | OpMul => pw_aff_from_aff (AVar res)
+    | OpLe => indicator_function (le_set (pw_aff_from_aff (AVar op1)) (pw_aff_from_aff (AVar op2)))
+    end.
+
+  Definition pmap_set_out_var_binop (m: PMap) (res: vid) (opc: BinArithOpCode) (op1 op2: vid) :=
+    let p2' := binop_to_pwaff res opc op1 op2 in
+    let c_map := Presburger.eq_map (pw_aff_from_aff (AConst 0)) (pw_aff_from_aff (AVar res)) (pw_aff_from_aff (AConst 0)) p2' in
+    let m_projected := map_project_out_out m res in
+    let new_map := intersect_map c_map m_projected in
+    new_map.
+
+  Theorem pmap_set_out_var_binop_spec (m: PMap) :
+    forall x0 x1, Ensembles.In _ (gamma m) (x0, x1) ->
+      forall res op1, res != op1 ->
+        forall op2, res != op2 ->
+          forall opc, Ensembles.In _ (gamma (pmap_set_out_var_binop m res opc op1 op2)) (x0, (res !-> bin_op_eval opc (x1 op1) (x1 op2); x1)).
+  Proof.
+    move => x0 x1 HIn res op1 Hop1 op2 Hop2 opc.
+    rewrite /gamma /= /gamma_pmap /Ensembles.In /pmap_set_out_var_binop /= /binop_to_pwaff.
+    case opc; simpl_presburger.
+    - apply map_project_out_out_spec.
+      exists (x1 res).
+        by auto_presburger.
+    - apply map_project_out_out_spec.
+      exists (x1 res).
+        by auto_presburger.
+    - case (_ <=? _)%Z; simplssr; apply map_project_out_out_spec; exists (x1 res); by auto_presburger.
+  Qed.
+
+  Theorem pmap_set_out_var_binop_tf_sound :
+    forall res opc op1 op2 Hop1 Hop2 R R',
+      inst_step (BinOp res opc op1 op2 Hop1 Hop2) R R' ->
+      forall m R_begin, Ensembles.In _ (gamma m) (R_begin, R) ->
+                   Ensembles.In _ (gamma (pmap_set_out_var_binop m res opc op1 op2)) (R_begin, R').
+  Proof.
+    move => res opc op1 op2 Hop1 Hop2 R R' Hinst m R_begin Hin.
+    by case: opc Hinst => Hinst; inversion Hinst; subst; apply pmap_set_out_var_binop_spec; autossr.
+  Qed.
+
+  Definition pmap_tf_inst (inst: Inst) (m: PMap) :=
+    match inst with
+    | Const res c => pmap_set_out_var_const m res c
+    | BinOp res opc op1 op2 op1_ne_res op2_ne_res => pmap_set_out_var_binop m res opc op1 op2
+    end.
+
+  Theorem pmap_tf_inst_sound :
+    forall inst R R',
+      inst_step inst R R' ->
+      forall m R_begin, Ensembles.In _ (gamma m) (R_begin, R) ->
+                   Ensembles.In _ (gamma (pmap_tf_inst inst m)) (R_begin, R').
+  Proof.
+    move => inst R R' Hinst m R_begin Hin.
+    case: inst Hinst => [ res v | res opc op1 op2 Hop1 Hop2 ] Hinst.
+    - eapply pmap_set_out_var_const_tf_sound; eauto.
+    - eapply pmap_set_out_var_binop_tf_sound; eauto.
+  Qed.
+
+  (* Transfer function for unconditional branch instruction *)
+  Fixpoint pmap_affect_variables (m: PMap) (vars inputs: list vid) :=
+    match (vars, inputs) with
+    | (nil, _) => m
+    | (_, nil) => m
+    | (var::vars', input::inputs') =>
+      if var == input then
+        pmap_affect_variables m vars' inputs'
+      else
+        let c_map := Presburger.eq_map (pw_aff_from_aff (AConst 0)) (pw_aff_from_aff (AVar var)) (pw_aff_from_aff (AConst 0)) (pw_aff_from_aff (AVar input)) in
+        let m_projected := map_project_out_out m var in
+        let new_m := intersect_map c_map m_projected in
+        pmap_affect_variables new_m vars' inputs'
+    end.
+
+  Theorem pmap_affect_variables_sound :
+    forall R_begin R m,
+      Ensembles.In _ (gamma m) (R_begin, R) ->
+      forall vars inputs, Ensembles.In _ (gamma (pmap_affect_variables m vars inputs)) (R_begin, affect_variables R vars inputs).
+  Proof.
+    move => R_begin R m Hin vars.
+    elim: vars R_begin R m Hin => [// | var vars Hind R_begin R m Hin inputs].
+    case: inputs => [ // | input inputs /=].
+    case (var =P input) => [ -> /= | ].
+    - apply Hind. rewrite /gamma /= /Ensembles.In /gamma_pmap /=. by auto_map.
+    - move => Hne. apply Hind. rewrite /gamma /= /Ensembles.In /gamma_pmap /=.
+      simpl_presburger. apply map_project_out_out_spec.
+      exists (R var). by auto_map.
+  Qed.
+
+  Definition pmap_tf_branch (out_id: bbid) (inputs: seq vid) (m: PMap) :=
+    [::(pmap_affect_variables m (get_inputs prog out_id) inputs, out_id)].
+
+  Theorem pmap_tf_branch_sound :
+    forall out_id inputs out_id' R R',
+      term_step prog (Br out_id inputs) R (out_id', R') ->
+      forall m R_begin, Ensembles.In _ (gamma m) (R_begin, R) ->
+                   exists m', ((m', out_id') \in (pmap_tf_branch out_id inputs m)) /\
+                         Ensembles.In  _ (gamma m') (R_begin, R').
+  Proof.
+    move => out_id inputs out_id' R R' Hterm m R_begin Hin.
+    inversion Hterm. subst.
+    eexists. split.
+    - rewrite mem_seq1. by apply eq_refl.
+    - by apply pmap_affect_variables_sound.
+  Qed.
+
+  Definition pmap_tf_branch_cond (cond: vid) (out_id_t: bbid) (inputs_t: seq vid) (out_id_f: bbid) (inputs_f: seq vid) (m: PMap) :=
+    let map_true := ne_map (pw_aff_from_aff (AConst 0)) (pw_aff_from_aff (AVar cond)) (pw_aff_from_aff (AConst 0)) (pw_aff_from_aff (AConst 0)) in
+    let map_true' := intersect_map map_true m in
+    let res_map_true := pmap_affect_variables map_true' (get_inputs prog out_id_t) inputs_t in
+    let map_false := Presburger.eq_map (pw_aff_from_aff (AConst 0)) (pw_aff_from_aff (AVar cond)) (pw_aff_from_aff (AConst 0)) (pw_aff_from_aff (AConst 0)) in
+    let map_false' := intersect_map map_false m in
+    let res_map_false := pmap_affect_variables map_false' (get_inputs prog out_id_f) inputs_f in
+    [::(res_map_true, out_id_t);(res_map_false, out_id_f)].
+
+  Theorem pmap_tf_branch_cond_sound :
+    forall cond out_id_t inputs_t out_id_f inputs_f out_id' R R',
+      term_step prog (BrC cond out_id_t inputs_t out_id_f inputs_f) R (out_id', R') ->
+      forall m R_begin, Ensembles.In _ (gamma m) (R_begin, R) ->
+                   exists m', ((m', out_id') \in (pmap_tf_branch_cond cond out_id_t inputs_t out_id_f inputs_f m)) /\
+                         Ensembles.In  _ (gamma m') (R_begin, R').
+  Proof.
+    move => cond out_id_t inputs_t out_id_f inputs_f out_id' R R' Hterm m R_begin HIn.
+    inversion Hterm; subst.
+    - eexists. split.
+      + rewrite in_cons. apply /orP. left. by apply eq_refl.
+      + apply pmap_affect_variables_sound.
+        rewrite /= /gamma_pmap /Ensembles.In. by auto_presburger.
+    - eexists. split.
+      + rewrite in_cons mem_seq1. apply /orP. right. by apply eq_refl.
+      + apply pmap_affect_variables_sound.
+        rewrite /= /gamma_pmap /Ensembles.In. simpl_presburger.
+        rewrite H6. by autossr.
+  Qed.
+
+  Definition pmap_tf_term (term: Term) (m: PMap) :=
+    match term with
+    | Br out_id inputs => pmap_tf_branch out_id inputs m
+    | BrC cond out_id_t inputs_t out_id_f inputs_f => pmap_tf_branch_cond cond out_id_t inputs_t out_id_f inputs_f m
+    end.
+
+  Theorem pmap_tf_term_sound :
+    forall term R bb R',
+      term_step prog term R (bb, R') ->
+      forall m R_begin, Ensembles.In _ (gamma m) (R_begin, R) ->
+                   exists m', ((m', bb) \in (pmap_tf_term term m)) /\
+                         Ensembles.In  _ (gamma m') (R_begin, R').
+  Proof.
+    move => term R bb R'. case term.
+    - intros. eapply pmap_tf_branch_sound; eauto.
+    - intros. eapply pmap_tf_branch_cond_sound; eauto.
+  Qed.
+
+  Instance tf_relational_pmap : transfer_function_relational adom_relational_pmap prog :=
+    {
+      transfer_inst := pmap_tf_inst;
+      transfer_inst_sound := pmap_tf_inst_sound;
+
+      transfer_term := pmap_tf_term;
+      transfer_term_sound := pmap_tf_term_sound;
+    }.
+  Admitted.
+
 
 End PMapAbstractDomain.
